PDL syntax

src/syntax.lean
@@ -25,7 +25,7 @@ infixr `⋏`:66        := formula.and
 @[simp]
 def impl (φ ψ : formula) := ~(φ ⋏ (~ψ))
 infixr `↣`:55        := impl
-infixl `⟷`:77        := λ ϕ ψ, (ϕ ↣ ψ) ⋏ (ψ ↣ ϕ)
+infixl `⟷`:77       := λ ϕ ψ, (ϕ ↣ ψ) ⋏ (ψ ↣ ϕ)
 
 @[simp]
 instance : has_bot formula := ⟨formula.bottom⟩
@@ -76,3 +76,96 @@ class hasComplexity (α : Type) := (complexityOf : α → ℕ)
 open hasComplexity
 instance formula_hasComplexity : hasComplexity formula := hasComplexity.mk complexityOfFormula
 instance setFormula_hasComplexity : hasComplexity (finset formula) := hasComplexity.mk complexityOfSet
+
+
+
+/- Syntax of PDL -/
+
+mutual inductive form, prog 
+with form : Type 
+| atom_form : char → form
+| neg : form → form
+| conj : form → form → form
+| box : prog → form → form
+with prog : Type
+| atom_prog : char → prog 
+| seq : prog → prog → prog 
+| star : prog → prog 
+| test : form → prog
+
+notation `#` p := form.atom_form p
+prefix `!`: 40 := form.neg 
+infixr `&&` : 50 := form.conj
+prefix `[]` : 42 := form.box
+notation `$` a : 40 := prog.atom_prog a
+infixr `;` : 48 := prog.seq
+-- the next two notation should appear at the end rather than the front, 
+-- but I cannot find the dual to "prefix"
+prefix `⋆` : 40 := prog.star
+prefix `?` : 40 := prog.test
+
+
+mutual def form_size, prog_size
+with form_size : form → nat 
+| (form.atom_form _) := 1
+| (form.neg φ)       := form_size φ + 1
+| (form.conj φ ψ)    := form_size φ + form_size ψ + 1
+| (form.box a φ)     := form_size φ + prog_size a  + 1
+with prog_size : prog → nat 
+| (prog.atom_prog _) := 1
+| (prog.seq a b)     := prog_size a + prog_size b + 1
+| (prog.star a)      := prog_size a + 1
+| (prog.test φ)      := form_size φ + 1
+
+
+lemma formatom : ∀ (p : char), 0 < form_size (# p) := 
+begin 
+  intro, unfold form_size, finish,
+end 
+
+lemma formneg { φ : form } : 0 < form_size φ → 0 < form_size (! φ) :=
+begin 
+  intro,unfold form_size, finish,
+end 
+
+lemma formconj { φ ψ : form } : 0 < form_size φ → 0 < form_size ψ → 0 < form_size (φ&&ψ) := 
+begin 
+  intros, unfold form_size, finish,
+end 
+
+lemma formbox { φ : form }{ a : prog } : 0 < form_size φ → 0 < prog_size a → 0 < form_size (([]a) φ) :=
+begin 
+  intros, unfold form_size, finish,
+end 
+
+lemma progatom : ∀ (a : char),  0 <  prog_size ($ a) := 
+begin 
+   intro, unfold prog_size, finish,
+end
+
+lemma progseq { a b : prog } : 0 < prog_size a → 0 < prog_size b →  0 < prog_size (a;b) :=
+begin 
+  intros, unfold prog_size, finish,
+end
+
+lemma progstar { a : prog } : 0 < prog_size a → 0 < prog_size (⋆a) :=
+begin 
+  intros, unfold prog_size, finish,
+end 
+
+lemma progtest { φ : form } : 0 < form_size φ → 0 < prog_size (?φ) :=
+begin 
+  intro, unfold prog_size, finish,
+end 
+
+mutual lemma fsize, psize
+with fsize : ∀ φ, 0 < form_size φ 
+| (# _)       := formatom _
+| (! φ)       := formneg (fsize φ)
+| (φ&&ψ)      := formconj (fsize φ) (fsize ψ)
+| (([]a) φ)   := formbox (fsize φ) (psize a)
+with psize :  ∀ a, 0 < prog_size a
+| ($ _)       := progatom _
+| (a ; b)     := progseq (psize a) (psize b)
+| (⋆a)        := progstar (psize a)
+| (?φ)        := progtest (fsize φ)
